rocq/Ender/Semantics.v
@@ -46,6 +46,7 @@ Definition statement_meaning (s : Statement) : Prop :=
   | PerpAt a b p =>
       Perp_at (point p) (point a.(seg_start)) (point a.(seg_end))
               (point b.(seg_start)) (point b.(seg_end))
+  | MidptOf s p => Midpoint (point p) (point s.(seg_start)) (point s.(seg_end))
   end.
 
 Definition segment_points (s : Segment) :=
